Simplify definition of ms_suffix (rely on standard library), integrate group nums into equiv relation, prove a technical lemma

warblreequiv/RegexpTranslation.v
@@ -5,7 +5,7 @@ Import Result.
 Import Result.Notations.
 Local Open Scope result_flow.
 
-Fixpoint to_warblre_regex (r: regex): Result Patterns.Regex CompileError :=
+(*Fixpoint to_warblre_regex (r: regex): Result Patterns.Regex CompileError :=
   match r with
   | Epsilon => Success Patterns.Empty
   | Character cd => char_descr_to_regex cd
@@ -23,7 +23,7 @@ Fixpoint to_warblre_regex (r: regex): Result Patterns.Regex CompileError :=
   | Group id r =>
     let! wr =<< to_warblre_regex r in
     Success (Patterns.Group None wr)
-  end.
+  end.*)
 
 (* Ensuring that the group IDs of the translation correspond to those of the original regexp *)
 Fixpoint num_groups (r: regex): nat :=
@@ -35,23 +35,20 @@ Fixpoint num_groups (r: regex): nat :=
   | Group _ r1 => S (num_groups r1)
   end.
 
-Inductive well_parenthesized' : nat -> regex -> Prop :=
-| wp_eps: forall n, well_parenthesized' n Epsilon
-| wp_char: forall n cd, well_parenthesized' n (Character cd)
-| wp_disj: forall n r1 r2, well_parenthesized' n r1 -> well_parenthesized' (num_groups r1 + n) r2 -> well_parenthesized' n (Disjunction r1 r2)
-| wp_seq: forall n r1 r2, well_parenthesized' n r1 -> well_parenthesized' (num_groups r1 + n) r2 -> well_parenthesized' n (Sequence r1 r2)
-| wp_star: forall n greedy r, well_parenthesized' n r -> well_parenthesized' n (Star greedy r)
-| wp_group: forall n r, well_parenthesized' (S n) r -> well_parenthesized' n (Group (S n) r).
 
-Definition well_parenthesized (r: regex) := well_parenthesized' 0 r.
+(* equiv_regex' wreg lreg n means that the two regexes wreg and lreg are equivalent, where the number of parentheses before wreg/lreg is n *)
+Inductive equiv_regex': Patterns.Regex -> regex -> nat -> Prop :=
+| Equiv_empty: forall n: nat, equiv_regex' Patterns.Empty Epsilon n
+| Equiv_char: forall (n: nat) (c: Char), equiv_regex' (Patterns.Char c) (Character (Chars.single c)) n
+| Equiv_dot: forall n: nat, equiv_regex' Patterns.Dot (Character Chars.dot) n
+| Equiv_disj: forall n wr1 wr2 lr1 lr2,
+    equiv_regex' wr1 lr1 n -> equiv_regex' wr2 lr2 (num_groups lr1 + n) ->
+    equiv_regex' (Patterns.Disjunction wr1 wr2) (Disjunction lr1 lr2) n
+| Equiv_seq: forall n wr1 wr2 lr1 lr2,
+    equiv_regex' wr1 lr1 n -> equiv_regex' wr2 lr2 (num_groups lr1 + n) ->
+    equiv_regex' (Patterns.Seq wr1 wr2) (Sequence lr1 lr2) n
+| Equiv_star_lazy: forall n wr lr, equiv_regex' wr lr n -> equiv_regex' (Patterns.Quantified wr (Patterns.Lazy Patterns.Star)) (Star false lr) n
+| Equiv_star_greedy: forall n wr lr, equiv_regex' wr lr n -> equiv_regex' (Patterns.Quantified wr (Patterns.Greedy Patterns.Star)) (Star true lr) n
+| Equiv_group: forall name n wr lr, equiv_regex' wr lr (S n) -> equiv_regex' (Patterns.Group name wr) (Group (S n) lr) n.
 
-
-Inductive equiv_regex: Patterns.Regex -> regex -> Prop :=
-| Equiv_empty: equiv_regex Patterns.Empty Epsilon
-| Equiv_char: forall c: Char, equiv_regex (Patterns.Char c) (Character (Chars.single c))
-| Equiv_dot: equiv_regex Patterns.Dot (Character Chars.dot)
-| Equiv_disj: forall wr1 wr2 r1 r2, equiv_regex wr1 r1 -> equiv_regex wr2 r2 -> equiv_regex (Patterns.Disjunction wr1 wr2) (Disjunction r1 r2)
-| Equiv_seq: forall wr1 wr2 r1 r2, equiv_regex wr1 r1 -> equiv_regex wr2 r2 -> equiv_regex (Patterns.Seq wr1 wr2) (Sequence r1 r2)
-| Equiv_star_lazy: forall wr r, equiv_regex wr r -> equiv_regex (Patterns.Quantified wr (Patterns.Lazy Patterns.Star)) (Star false r)
-| Equiv_star_greedy: forall wr r, equiv_regex wr r -> equiv_regex (Patterns.Quantified wr (Patterns.Greedy Patterns.Star)) (Star true r)
-| Equiv_group: forall name wr gid r, equiv_regex wr r -> equiv_regex (Patterns.Group name wr) (Group gid r).
+Definition equiv_regex (wreg: Patterns.Regex) (lreg: regex) := equiv_regex' wreg lreg 0.
